Steel.Repr.M: vprop lists

experiment/Experiment.Steel.Repr.M.fst
@@ -1,44 +1,489 @@
 module Experiment.Steel.Repr.M
 
+module T    = FStar.Tactics
+module U    = Learn.Util
+module L    = FStar.List.Pure
+module Uv   = FStar.Universe
+module Ll   = Learn.List
+module Mem  = Steel.Memory
+module Perm = Learn.Permutation
+module FExt = FStar.FunctionalExtensionality
+
+open FStar.Calc
+open FStar.Classical.Sugar
+
 open Steel.Effect
 open Steel.Effect.Atomic
-open Steel.Reference
 
 #set-options "--ide_id_info_off"
 
 irreducible let __tree_reduce__ : unit = ()
 
-assume val some_ref : ref nat
-unfold let vp = vptr some_ref
-let sl_t = Ghost.erased nat
-type req_t = sl_t -> prop
-type ens_t (a : Type) = sl_t -> a -> sl_t -> prop
-type repr_steel_t (a : Type) (req : req_t) (ens : ens_t a) : Type
-  = unit -> Steel a vp (fun _ -> vp) (requires fun h0 -> req (h0 vp)) (ensures fun h0 x h1 -> ens (h0 vp) x (h1 vp))
+(** [var_list] *)
+
+(* ALT? dependent arrrow Fin.fin n -> _ *)
+
+type ty_list = list Type
 
 noeq
-type prog_tree : (a : Type u#a) -> Type u#(a+1) =
-  | Tspec  : (a : Type) -> (req : req_t) -> (ens : ens_t a) ->
+type var_list : ty_list -> Type =
+  | VLNil : var_list []
+  | VLCons : (t0 : Type) -> (x0 : t0) ->
+             (ts : ty_list) -> (xs : var_list ts) ->
+             var_list (t0 :: ts)
+
+let rec var_at (#ts : ty_list) (xs : var_list ts) (i : nat{i < L.length ts})
+  : L.index ts i
+  = let VLCons t0 x0 ts1 xs1 = xs in
+    if i = 0 then x0
+    else U.cast (L.index ts i) (var_at xs1 (i-1))
+
+let rec var_list_extensionality (#ts : ty_list) (xs ys : var_list ts)
+  : Lemma (requires forall (i : nat {i < L.length ts}) . var_at xs i == var_at ys i)
+          (ensures xs == ys)
+          (decreases ts)
+  = match ts with
+    | [] -> ()
+    | t0 :: ts' -> let VLCons _ x _ xs' = xs in
+                let VLCons _ y _ ys' = ys in
+                assert (x == var_at xs 0);
+                assert (y == var_at ys 0);
+                introduce forall (i : nat {i < L.length ts'}) . var_at xs' i == var_at ys' i
+                  with (assert (var_at xs' i === var_at xs (i+1));
+                        assert (var_at ys' i === var_at ys (i+1)));
+                var_list_extensionality #ts' xs' ys'
+
+let rec var_splitAt (n : nat) (#ts : ty_list) (xs : var_list ts)
+  : Tot (var_list (L.splitAt n ts)._1 & var_list (L.splitAt n ts)._2)
+        (decreases n)
+  = if n = 0 then VLNil, xs
+    else match xs with
+    | VLNil              -> VLNil, VLNil
+    | VLCons t0 x0 ts xs -> let xs0, xs1 = var_splitAt (n-1) xs in
+                           VLCons t0 x0 _ xs0, xs1
+
+let rec var_initi (lb ub : nat)
+          (t : (i:nat{lb <= i /\ i < ub}) -> Tot Type)
+          (f : (i:nat{lb <= i /\ i < ub}) -> Tot (t i))
+  : Tot (var_list (Ll.initi lb ub t)) (decreases ub - lb)
+  = if lb < ub then VLCons (t lb) (f lb) _ (var_initi (lb + 1) ub t f) else VLNil
+
+let rec var_initi_at (lb ub : nat)
+          (t : (i:nat{lb <= i /\ i < ub}) -> Tot Type)
+          (f : (i:nat{lb <= i /\ i < ub}) -> Tot (t i))
+          (i : nat {i < L.length (Ll.initi lb ub t)})
+  : Lemma (ensures var_at (var_initi lb ub t f) i == f (lb+i)) (decreases i)
+          [SMTPat (var_at (var_initi lb ub t f) i)]
+  = if i = 0 then () else var_initi_at (lb+1) ub t f (i-1)
+
+let var_apply_perm_r (#n : nat) (p : Perm.perm_f n) (#ts : ty_list {L.length ts == n}) (xs : var_list ts)
+  : var_list (Perm.apply_perm_r p ts)
+  = var_initi 0 n (fun i -> L.index ts (p i)) (fun i -> var_at xs (p i))
+
+let var_apply_r_id_n (len : nat) (#ts : ty_list{L.length ts = len}) (xs :var_list ts)
+  : Lemma (var_apply_perm_r (Perm.id_n len) xs == xs) [SMTPat (var_apply_perm_r (Perm.id_n len) xs)]
+  = var_list_extensionality (var_apply_perm_r (Perm.id_n len) xs) xs
+
+let var_apply_r_comp (#len : nat) (f g : Perm.perm_f len) (#ts : ty_list {L.length ts == len}) (xs : var_list ts)
+  : Lemma (var_apply_perm_r (f `Perm.comp` g) xs === var_apply_perm_r f (var_apply_perm_r g xs))
+  = Perm.apply_r_comp f g ts;
+    var_list_extensionality (var_apply_perm_r (f `Perm.comp` g) xs) (var_apply_perm_r f (var_apply_perm_r g xs))
+
+let rec var_list_swap (i : nat) (#ts : ty_list{i <= L.length ts - 2}) (xs : var_list ts)
+  : Tot (var_list (Perm.list_swap i ts)) (decreases i)
+  = if i = 0
+    then let VLCons tx x _ (VLCons ty y _ tl) = xs in
+         VLCons ty y _ (VLCons tx x _ tl)
+    else let VLCons tx x ts tl = xs in
+         VLCons tx x _ (var_list_swap (i-1) tl)
+
+#push-options "--z3rlimit 20"
+let var_apply_perm_f_shift (#len : nat) (p : Perm.perm_f len)
+      (#hd_ty : Type) (#tl_ty : ty_list {L.length tl_ty = len})
+      (hd : hd_ty) (tl : var_list tl_ty)
+  : Lemma (var_apply_perm_r (Perm.perm_f_shift p) (VLCons _ hd _ tl)
+       === VLCons _ hd _ (var_apply_perm_r p tl))
+  = Perm.apply_perm_f_shift p hd_ty tl_ty;
+    var_list_extensionality
+      (var_apply_perm_r (Perm.perm_f_shift p) (VLCons _ hd _ tl))
+      (VLCons _ hd _ (var_apply_perm_r p tl))
+#pop-options
+
+#push-options "--z3rlimit 60"
+let rec var_apply_swap_as_rec (len : nat) (i : nat {i <= len-2})
+          (#ts : ty_list {L.length ts = len}) (xs : var_list ts)
+  : Lemma (ensures var_apply_perm_r (Perm.perm_f_swap #len i) xs === var_list_swap i xs)
+          (decreases len)
+  = Perm.apply_swap_as_rec len i ts;
+    if i = 0 then begin
+       let VLCons _ x _ (VLCons _ y _ tl) = xs in
+       var_list_extensionality
+         (var_apply_perm_r (Perm.perm_f_swap #len 0) (VLCons _ x _ (VLCons _ y _ tl)))
+         (VLCons _ y _ (VLCons _ x _ tl))
+    end else begin
+      let VLCons _ hd _ tl = xs in
+      Perm.perm_f_swap_rec_rel (len-1) (i-1);
+      var_apply_perm_f_shift (Perm.perm_f_swap #(len-1) (i-1)) hd tl;
+      var_apply_swap_as_rec (len-1) (i-1) tl
+    end
+#pop-options
+
+
+(** [vprop_list] *)
+
+type vprop_list = list vprop'
+
+let rec vprop_of_list (vpl : vprop_list) : vprop =
+  match vpl with
+  | [] -> emp
+  | v :: vs -> VStar (VUnit v) (vprop_of_list vs)
+
+let rec vprop_of_list_can_be_split (vs : vprop_list) (i : nat {i < L.length vs})
+  : Lemma (ensures can_be_split (vprop_of_list vs) (VUnit (L.index vs i)))
+  = let v :: vs = vs in
+    if i = 0
+    then can_be_split_star_l (VUnit v) (vprop_of_list vs)
+    else begin
+      can_be_split_star_r (VUnit v) (vprop_of_list vs);
+      vprop_of_list_can_be_split vs (i-1);
+      can_be_split_trans (VUnit v `star` vprop_of_list vs) (vprop_of_list vs) (VUnit (L.index vs (i-1)))
+    end
+
+let rec flatten_vprop_aux (vp : vprop) (acc : vprop_list) : GTot vprop_list =
+  match vp with
+  | VUnit vp' -> vp' :: acc
+  | VStar vp0 vp1 -> flatten_vprop_aux vp0 (flatten_vprop_aux vp1 acc)
+
+let flatten_vprop (vp : vprop) : GTot vprop_list = flatten_vprop_aux vp []
+
+let rec flatten_vprop_aux_eq (vp : vprop) (acc : vprop_list)
+  : Lemma (flatten_vprop_aux vp acc == L.(flatten_vprop vp @ acc))
+  = match vp with
+  | VUnit _ -> ()
+  | VStar vp0 vp1 ->
+          calc (==) {
+            flatten_vprop_aux (VStar vp0 vp1) acc;
+          == {}
+            flatten_vprop_aux vp0 (flatten_vprop_aux vp1 acc);
+          == {flatten_vprop_aux_eq vp0 (flatten_vprop_aux vp1 acc);
+              flatten_vprop_aux_eq vp1 acc}
+            L.(flatten_vprop vp0 @ (flatten_vprop vp1 @ acc));
+          == {L.append_assoc (flatten_vprop vp0) (flatten_vprop vp1) acc}
+            L.((flatten_vprop vp0 @ (flatten_vprop vp1 @ [])) @ acc);
+          == {flatten_vprop_aux_eq vp1 [];
+              flatten_vprop_aux_eq vp0 (flatten_vprop_aux vp1 [])}
+            L.(flatten_vprop_aux (VStar vp0 vp1) [] @ acc);
+          }
+
+let flatten_vprop_VStar (vp0 vp1 : vprop)
+  : Lemma (flatten_vprop (VStar vp0 vp1) == L.(flatten_vprop vp0 @ flatten_vprop vp1))
+  =
+    flatten_vprop_aux_eq vp0 (flatten_vprop_aux vp1 []);
+    flatten_vprop_aux_eq vp1 []
+
+let rec vprop_of_list_append (vs0 vs1 : vprop_list)
+  : Lemma (ensures equiv (vprop_of_list L.(vs0@vs1)) (vprop_of_list vs0 `star` vprop_of_list vs1))
+          (decreases vs0)
+  = match vs0 with
+  | []     -> assert (equiv (vprop_of_list vs1) (emp `star` vprop_of_list vs1))
+                by (init_resolve_tac ())
+  | v :: vs -> let v0 = VUnit v in
+             let vl0 = vprop_of_list vs in
+             let vl1 = vprop_of_list vs1 in
+             let vl2 = vprop_of_list L.(vs @ vs1) in
+             assert_norm (vprop_of_list L.((v :: vs) @ vs1) == v0 `star` vl2);
+             equiv_refl v0;
+             vprop_of_list_append vs vs1;
+             star_congruence v0       vl2
+                             v0 (vl0 `star` vl1);
+             star_associative v0 vl0 vl1;
+             equiv_sym ((v0 `star` vl0) `star` vl1) (v0 `star` (vl0 `star` vl1));
+             
+             equiv_trans (v0 `star` vl2)
+                         (v0 `star` (vl0 `star` vl1))
+                         ((v0 `star` vl0) `star` vl1);
+             assert_norm (vprop_of_list (v :: vs) `star` vprop_of_list vs1
+                      == (v0 `star` vl0) `star` vl1)
+
+let rec vprop_equiv_flat (vp : vprop)
+  : Lemma (equiv (vprop_of_list (flatten_vprop vp)) vp)
+  = match vp with
+  | VUnit v     -> assert (equiv (VUnit v `star` emp) (VUnit v))
+                      by (init_resolve_tac ())
+  | VStar v0 v1 -> flatten_vprop_VStar v0 v1;
+                  vprop_of_list_append (flatten_vprop v0) (flatten_vprop v1);
+                  vprop_equiv_flat v0;
+                  vprop_equiv_flat v1;
+                  star_congruence (vprop_of_list (flatten_vprop v0)) (vprop_of_list (flatten_vprop v1)) v0 v1;
+                  equiv_trans (vprop_of_list L.(flatten_vprop v0 @ flatten_vprop v1))
+                              (vprop_of_list (flatten_vprop v0) `star` vprop_of_list (flatten_vprop v1))
+                              (v0 `star` v1)
+
+
+let vprop_list_sels_t : vprop_list -> ty_list =
+  L.map (fun (vp:vprop') -> vp.t) 
+
+unfold
+let sl_t (vs : vprop_list) : Type = var_list (vprop_list_sels_t vs)
+
+let vprop_list_sels_t_eq (vs : vprop_list) (i : nat {i < L.length vs})
+  : Lemma (ensures L.index (vprop_list_sels_t vs) i == (L.index vs i).t)
+          [SMTPat (L.index (vprop_list_sels_t vs) i)]
+  = Ll.map_index (fun (vp:vprop') -> vp.t) vs i
+
+let rec vpl_sels (vs : vprop_list) (sl : t_of (vprop_of_list vs))
+  : Tot (sl_t vs) (decreases vs)
+  = match (|vs, sl|) <: (vs : vprop_list & t_of (vprop_of_list vs))  with
+  | (|[], _|) -> VLNil
+  | (|v0 :: vs, (x0, xs)|) -> VLCons v0.t x0 _ (vpl_sels vs xs)
+
+unfold
+let rmem_sels (#p:vprop) (vs : vprop_list)
+    (h:rmem p{FStar.Tactics.with_tactic selector_tactic (can_be_split p (vprop_of_list vs) /\ True)})
+  : GTot (sl_t vs)
+  = vpl_sels vs (h (vprop_of_list vs))
+
+(*
+let rec rmem_sels (vs : vprop_list) (h : rmem (vprop_of_list vs))
+  : GTot (var_list (vprop_list_sels_t vs)) (decreases vs)
+  = match vs with
+  | []     -> VLNil
+  | v :: vs -> let _ : (can_be_split (vprop_of_list (v :: vs)) (VUnit v) /\ True) = _
+                 by (T.norm [iota; zeta; delta_only [`%vprop_of_list]]; selector_tactic ()) in
+              let _ : (can_be_split (vprop_of_list (v :: vs)) (vprop_of_list vs) /\ True) = _
+                 by (T.norm [iota; zeta; delta_only [`%vprop_of_list]]; selector_tactic ()) in
+              VLCons v.t (h (VUnit v)) _ (rmem_sels vs (focus_rmem h (vprop_of_list vs)))
+
+let focus_rmem_feq (p q r : vprop) (h : rmem p)
+  : Lemma (requires can_be_split p q /\ can_be_split q r)
+          (ensures  can_be_split p r /\ focus_rmem h q r == h r)
+  = can_be_split_trans p q r
+
+let rec rmem_sels_eq (vs : vprop_list) (h : rmem (vprop_of_list vs)) (i : nat {i < L.length vs})
+  : Lemma (ensures vprop_of_list_can_be_split vs i;
+                  (var_at (rmem_sels vs h) i == h (VUnit (L.index vs i))))
+  = let v :: vs' = vs in
+    if i = 0 then ()
+    else begin
+      let _ : (can_be_split (vprop_of_list (v :: vs')) (vprop_of_list vs') /\ True) = _
+         by (T.norm [iota; zeta; delta_only [`%vprop_of_list]]; selector_tactic ()) in
+      U.f_equal (fun vs -> rmem (vprop_of_list vs)) vs (v :: vs');
+      vprop_of_list_can_be_split vs' (i-1);
+      focus_rmem_feq (vprop_of_list (v :: vs')) (vprop_of_list vs') (VUnit (L.index vs' (i-1)))
+                     (U.cast (rmem (vprop_of_list (v :: vs'))) h);
+      rmem_sels_eq vs' (focus_rmem h (vprop_of_list vs')) (i-1)
+  end
+*)
+
+unfold
+let split_vars (vs0 vs1 : vprop_list) (xs : sl_t (vs0@vs1))
+  : sl_t vs0 & sl_t vs1
+  =
+    Ll.map_append (fun (vp:vprop') -> vp.t) vs0 vs1;
+    L.lemma_append_splitAt (vprop_list_sels_t vs0) (vprop_list_sels_t vs1);
+    var_splitAt (L.length vs0) xs
+ 
+
+let rec steel_elim_vprop_of_list_append #opened (vs0 vs1 : vprop_list)
+  : SteelGhost unit opened
+      (vprop_of_list L.(vs0@vs1)) (fun () -> vprop_of_list vs0 `star` vprop_of_list vs1)
+      (requires fun _ -> True)
+      (ensures fun h0 () h1 -> split_vars vs0 vs1 (rmem_sels (vs0@vs1) h0) == (rmem_sels vs0 h1, rmem_sels vs1 h1))
+      (decreases vs0)
+  = match vs0 with
+    | [] -> change_equal_slprop (vprop_of_list L.(vs0@vs1)) (vprop_of_list vs1);
+           change_equal_slprop emp (vprop_of_list vs0)
+    | v0 :: vs0' ->
+           change_equal_slprop (vprop_of_list L.(vs0@vs1)) (VUnit v0 `star` vprop_of_list L.(vs0'@vs1));
+           steel_elim_vprop_of_list_append vs0' vs1;
+           change_equal_slprop (VUnit v0 `star` vprop_of_list vs0') (vprop_of_list (vs0))
+
+let rec steel_intro_vprop_of_list_append #opened (vs0 vs1 : vprop_list)
+  : SteelGhost unit opened
+      (vprop_of_list vs0 `star` vprop_of_list vs1) (fun () -> vprop_of_list L.(vs0@vs1))
+      (requires fun _ -> True)
+      (ensures fun h0 () h1 -> split_vars vs0 vs1 (rmem_sels (vs0@vs1) h1) == (rmem_sels vs0 h0, rmem_sels vs1 h0))
+      (decreases vs0)
+  = match vs0 with
+    | [] -> change_equal_slprop (vprop_of_list vs0) emp;
+           change_equal_slprop (vprop_of_list vs1) (vprop_of_list L.(vs0@vs1))
+    | v0 :: vs0' ->
+           change_equal_slprop (vprop_of_list (vs0)) (VUnit v0 `star` vprop_of_list vs0');
+           steel_intro_vprop_of_list_append vs0' vs1;
+           change_equal_slprop (VUnit v0 `star` vprop_of_list L.(vs0'@vs1)) (vprop_of_list L.(vs0@vs1))
+           
+
+(** [vequiv] *)
+
+let vequiv (vs0 vs1 : vprop_list) : Type
+  = f : Perm.perm_f (L.length vs0) {vs1 == Perm.apply_perm_r f vs0}
+
+let vequiv_sels_t (#vs0 #vs1 : vprop_list) (f : vequiv vs0 vs1)
+  : Lemma (vprop_list_sels_t vs1 == Perm.apply_perm_r f (vprop_list_sels_t vs0))
+  = Perm.map_apply_r f (fun (vp:vprop') -> vp.t) vs0
+
+unfold
+let extract_vars (#src #dst : vprop_list)
+                 (p : vequiv src dst)
+                 (xs : sl_t src)
+  : sl_t dst
+  =
+    vequiv_sels_t p;
+    var_apply_perm_r p xs
+
+unfold
+let extract_vars_f (src dst frame : vprop_list)
+                   (p : vequiv src L.(dst@frame))
+                   (xs : sl_t src)
+  : sl_t dst & sl_t frame
+  =
+    split_vars dst frame (extract_vars p xs)
+
+unfold
+let vequiv_sym (#vs0 #vs1 : vprop_list) (f : vequiv vs0 vs1) : vequiv vs1 vs0
+  = 
+    Perm.(calc (==) {
+      apply_perm_r (inv_f f) vs1;
+    == {}
+      apply_perm_r (inv_f f) (apply_perm_r f vs0);
+    == {apply_r_comp (inv_f f) f vs0}
+      vs0;
+    });
+    U.cast #(Perm.perm_f (L.length vs0)) (Perm.perm_f (L.length vs1)) (Perm.inv_f f)
+
+let extract_vars_sym_l (#vs0 #vs1 : vprop_list) (f : vequiv vs0 vs1) (xs : sl_t vs0)
+  : Lemma (extract_vars (vequiv_sym f) (extract_vars f xs) == xs)
+  =
+    vequiv_sels_t f; vequiv_sels_t (vequiv_sym f);
+    calc (==) {
+      extract_vars (vequiv_sym f) (extract_vars f xs);
+    == {}
+      var_apply_perm_r (vequiv_sym f) (var_apply_perm_r f xs);
+    == {}
+      var_apply_perm_r (Perm.inv_f f) (var_apply_perm_r f xs);
+    == {var_apply_r_comp #(L.length vs0) (Perm.inv_f f) f xs}
+      xs;
+    }
+
+/// applying a permutation on the context's vprop
+
+let rec steel_change_swap (#opened:Mem.inames)
+          (vs0 : vprop_list) (i : nat {i <= L.length vs0 - 2})
+  : SteelGhost unit opened (vprop_of_list vs0) (fun () -> vprop_of_list (Perm.list_swap i vs0))
+      (requires fun _ -> True) (ensures fun h0 () h1 ->
+        rmem_sels (Perm.list_swap i vs0) h1 === var_list_swap i (rmem_sels vs0 h0))
+      (decreases i)
+  = if i = 0
+    then begin
+      let v0 :: v1 :: vs = vs0 in
+      change_equal_slprop (vprop_of_list vs0)
+                          (VUnit v0 `star` (VUnit v1 `star` vprop_of_list vs));
+      change_equal_slprop (VUnit v1 `star` (VUnit v0 `star` vprop_of_list vs))
+                          (vprop_of_list (Perm.list_swap i vs0))
+    end else begin
+      let v0 :: vs = vs0 in
+      change_equal_slprop (vprop_of_list vs0)
+                          (VUnit v0 `star` vprop_of_list vs);
+      steel_change_swap vs (i-1);
+      change_equal_slprop (VUnit v0 `star` vprop_of_list (Perm.list_swap (i-1) vs))
+                          (vprop_of_list (Perm.list_swap i vs0))
+    end
+
+let rec steel_change_vequiv_aux (#opened:Mem.inames)
+          (n : nat) (vs0 vs1 : (l:vprop_list{L.length l == n}))
+          (fs : list (i:nat{i <= n-2}))
+          (eqv : squash (vs1 == Perm.apply_perm_r (Perm.comp_list (L.map (Perm.perm_f_swap #n) fs)) vs0))
+  : SteelGhost unit opened (vprop_of_list vs0) (fun () -> vprop_of_list vs1)
+      (requires fun _ -> True) (ensures fun h0 () h1 ->
+        rmem_sels vs1 h1 == extract_vars (Perm.comp_list (L.map Perm.perm_f_swap fs)) (rmem_sels vs0 h0))
+      (decreases fs)
+  =
+  let sl0  = gget (vprop_of_list vs0) in
+  match fs with
+  | []       -> change_equal_slprop (vprop_of_list vs0) (vprop_of_list vs1)
+  | f0 :: fs' -> let pfs = Perm.comp_list (L.map (Perm.perm_f_swap #n) fs') in
+               let vs' = Perm.apply_perm_r pfs vs0 in
+               steel_change_vequiv_aux n vs0 vs' fs' ();
+               let sl1' = extract_vars #vs0 #vs' (U.cast (Perm.perm_f (L.length vs0)) pfs)
+                                                 (vpl_sels vs0 sl0) in
+               steel_change_swap vs' f0;
+               Perm.apply_swap_as_rec n f0 vs';
+               Perm.apply_r_comp (Perm.perm_f_swap #n f0) pfs vs0;
+               change_equal_slprop (vprop_of_list (Perm.list_swap f0 vs'))
+                                   (vprop_of_list vs1);
+               let sl1  = gget (vprop_of_list vs1) in
+               assert (vpl_sels vs1 sl1 === var_list_swap f0 sl1');
+               var_apply_swap_as_rec n f0 sl1';
+               var_apply_r_comp (Perm.perm_f_swap #n f0) pfs (vpl_sels vs0 sl0)
+
+let steel_change_vequiv (#vs0 #vs1 : vprop_list) (#opened:Mem.inames) (f : vequiv vs0 vs1)
+  : SteelGhost unit opened (vprop_of_list vs0) (fun () -> vprop_of_list vs1)
+      (requires fun _ -> True)
+      (ensures fun h0 () h1 -> rmem_sels vs1 h1 == extract_vars f (rmem_sels vs0 h0))
+  =
+    steel_change_vequiv_aux (L.length vs0) vs0 vs1 (Perm.perm_f_to_swap f) ()
+
+
+(*** [prog_tree] *)
+
+let pre_t = vprop_list
+let post_t (a : Type) = a -> vprop_list
+type req_t (pre : pre_t) = sl_t pre -> prop
+type ens_t (pre : pre_t) (a : Type) (post : post_t a) = sl_t pre -> (x : a) -> sl_t (post x) -> prop
+
+type repr_steel_t (a : Type)
+       (pre : pre_t) (post : post_t a)
+       (req : req_t pre) (ens : ens_t pre a post) : Type
+  = unit -> Steel a
+             (vprop_of_list pre) (fun x -> vprop_of_list (post x))
+             (requires fun h0      -> req (rmem_sels pre h0))
+             (ensures  fun h0 x h1 -> ens (rmem_sels pre h0) x (rmem_sels (post x) h1))
+
+noeq
+type prog_tree : (a : Type u#a) -> Type u#(max (a+1) 2) =
+  | Tspec  : (a : Type u#a) -> (pre : pre_t) -> (post : post_t a) ->
+             (req : req_t pre) -> (ens : ens_t pre a post) ->
              prog_tree a
-  | Tret   : (a : Type) -> (x : a) -> prog_tree a
+  | Tret   : (a : Type u#a) -> (x : a) -> prog_tree a
   | Tbind  : (a : Type u#a) -> (b : Type u#a) ->
              (f : prog_tree a) -> (g : a -> prog_tree b) ->
              prog_tree b
-  | TbindP : (a : Type u#a) -> (b : Type) ->
+  | TbindP : (a : Type u#a) -> (b : Type u#a) ->
              (wp : pure_wp a) -> (x : unit -> PURE a wp) -> (g : a -> prog_tree b) ->
              prog_tree b
 
+
+(*** slprop unification conditions *)
+
+(* TODO:
+   - ? equalities vs vequiv
+      + Tspec : post x == post' x @ frame, allow shuffle at the end
+   - ~pr ! allow assumptions -> VC
+   - ALT: datatype indexed by t *)
+
+let rec tree_cond (#a : Type u#a ) (t : prog_tree a) (pre : pre_t) (post : post_t a)
+  : Tot (Type u#(max a 2)) (decreases t)
+  = match t with
+  | Tspec a pre' post' _ _ ->
+          frame : vprop_list & vequiv pre L.(pre' @ frame)
+                             & ((x:a) -> vequiv (post' x @ frame) (post x))
+  | Tret  a x ->
+          Uv.raise_t u#0 u#(max a 2) (vequiv pre (post x))
+  | Tbind a b f g ->
+          itm : (a -> vprop_list) & tree_cond f pre itm & ((x:a) -> tree_cond (g x) (itm x) post)
+  | TbindP a b _ _ g ->
+          (x:a) -> tree_cond (g x) pre post
 
 (*** requires / ensures *)
 
 (** return *)
 
 unfold
-let return_req : req_t
+let return_req (pre : pre_t) : req_t pre
   = fun _ -> True
 
 unfold
-let return_ens (#a : Type) (x : a) : ens_t a
+let return_ens (#a : Type) (x : a) (p : a -> vprop_list) : ens_t (p x) a p
   = fun sl0 r sl1 ->
       r == x /\ sl1 == sl0
 
@@ -46,21 +491,23 @@ let return_ens (#a : Type) (x : a) : ens_t a
 
 unfold
 let bind_req (#a : Type)
-      (req_f : req_t) (ens_f : ens_t a)
-      (req_g : a -> req_t)
-  : req_t
+      (#pre : pre_t) (#itm : a -> vprop_list)
+      (req_f : req_t pre) (ens_f : ens_t pre a itm)
+      (req_g : (x:a) -> req_t (itm x))
+  : req_t pre
   = fun sl0 -> req_f sl0 /\
-      (forall (x : a) (sl1 : sl_t) .
+      (forall (x : a) (sl1 : sl_t (itm x)) .
         ens_f sl0 x sl1 ==> req_g x sl1)
 
 unfold
 let bind_ens (#a : Type) (#b : Type)
-      (req_f : req_t) (ens_f : ens_t a)
-      (ens_g : a -> ens_t b)
-  : ens_t b
+      (#pre : pre_t) (#itm : a -> vprop_list) (#post : post_t b)
+      (req_f : req_t pre) (ens_f : ens_t pre a itm)
+      (ens_g : (x:a) -> ens_t (itm x) b post)
+  : ens_t pre b post
   = fun sl0 y sl2 ->
       req_f sl0 /\
-      (exists (x : a) (sl1 : sl_t) .
+      (exists (x : a) (sl1 : sl_t (itm x)) .
         ens_f sl0 x sl1 /\
         ens_g x sl1 y sl2)
 
@@ -68,33 +515,55 @@ let bind_ens (#a : Type) (#b : Type)
 
 unfold
 let bind_pure_req (#a : Type) (wp : pure_wp a)
-      (req : a -> req_t)
-  : req_t
+      (#pre : pre_t)
+      (req : a -> req_t pre)
+  : req_t pre
   = fun sl0 -> wp (fun x -> req x sl0) /\ True
 
 unfold
 let bind_pure_ens (#a : Type) (#b : Type)
       (wp : pure_wp a)
-      (ens : a -> ens_t b)
-  : ens_t b
+      (#pre : pre_t) (#post : post_t b)
+      (ens : a -> ens_t pre b post)
+  : ens_t pre b post
   = fun sl0 y sl1 -> as_requires wp /\ (exists (x:a) . as_ensures wp x /\ ens x sl0 y sl1)
+
 
 (** prog_tree *)
 
-let rec tree_req (#a : Type) (r : prog_tree a)
-  : Tot req_t (decreases r) =
-  match r with
-  | Tspec  _ req _    -> req
-  | Tret   _ _        -> return_req
-  | Tbind  _ _ f g    -> bind_req (tree_req f) (tree_ens f) (fun x -> tree_req (g x))
-  | TbindP _ _ wp _ g -> bind_pure_req wp (fun x -> tree_req (g x))
-and tree_ens (#a : Type) (r : prog_tree a)
-  : Tot (ens_t a) (decreases r) =
-  match r with
-  | Tspec  _ _ ens    -> ens
-  | Tret   _ x        -> return_ens x
-  | Tbind  _ _ f g    -> bind_ens (tree_req f) (tree_ens f) (fun x -> tree_ens (g x))
-  | TbindP _ _ wp _ g -> bind_pure_ens wp (fun x -> tree_ens (g x))
+let rec tree_req (#a : Type u#a) (t : prog_tree a)
+                 (#pre : pre_t) (#post : post_t a) (c : tree_cond t pre post)
+  : Tot (req_t pre) (decreases t) =
+  let tc : (t : prog_tree a & tree_cond t pre post) = (|t, c|) in
+  match tc with
+  | (|Tspec  _ pre' _ req _, (|frame, p0, _|)|) ->
+             (fun sl0 -> req (extract_vars_f pre pre' frame p0 sl0)._1)
+  | (|Tret   _ _, _|) ->
+             return_req pre
+  | (|Tbind  _ _ f g, (|itm, cf, cg|)|) ->
+             bind_req (tree_req f cf) (tree_ens f cf) (fun x -> tree_req (g x) (cg x))
+  | (|TbindP _ _ wp _ g, cg|) ->
+             bind_pure_req wp (fun x -> tree_req (g x) (cg x))
+
+and tree_ens (#a : Type u#a) (t : prog_tree a)
+             (#pre : pre_t) (#post : post_t a) (c : tree_cond t pre post)
+  : Tot (ens_t pre a post) (decreases t) =
+  let tc : (t : prog_tree a & tree_cond t pre post) = (|t, c|) in
+  match tc with
+  | (|Tspec  a pre' post' req ens, (|frame, p0, p1|)|) ->
+             (fun sl0 x sl1 ->
+                let sl0', frame0 = extract_vars_f pre  pre'  frame p0 sl0 in
+                let sl1', frame1 = extract_vars_f (post x) (post' x) frame (vequiv_sym (p1 x)) sl1 in
+                frame1 == frame0 /\ ens sl0' x sl1')
+  | (|Tret   _ x, p|) ->
+             (fun sl0 x' sl1 ->
+                x' == x /\
+               (let sl0' = extract_vars #pre #(post x) (Uv.downgrade_val u#0 u#(max a 2) p) sl0 in
+                sl1 == sl0'))
+  | (|Tbind  _ _ f g, (|itm, cf, cg|)|) ->
+             bind_ens (tree_req f cf) (tree_ens f cf) (fun x -> tree_ens (g x) (cg x))
+  | (|TbindP _ _ wp _ g, cg|) ->
+             bind_pure_ens wp (fun x -> tree_ens (g x) (cg x))
 
 
 (*** "Monad" *)
@@ -105,19 +574,33 @@ and tree_ens (#a : Type) (r : prog_tree a)
 noeq
 type repr (a : Type) = {
   repr_tree  : prog_tree a;
-  repr_steel : repr_steel_t a (tree_req repr_tree) (tree_ens repr_tree)
+  repr_steel : (pre : pre_t) -> (post : post_t a) -> (c : tree_cond repr_tree pre post) ->
+               repr_steel_t a pre post (tree_req repr_tree c) (tree_ens repr_tree c)
 }
 
-let tree_of_steel (#a : Type) (#req : req_t) (#ens : ens_t a) ($f : repr_steel_t a req ens)
+let tree_of_steel (#a : Type) (#pre : pre_t) (#post : post_t a) (#req : req_t pre) (#ens : ens_t pre a post)
+                  ($f : repr_steel_t a pre post req ens)
   : prog_tree a
-  = Tspec a req ens
+  = Tspec a pre post req ens
+
 
 [@@ __tree_reduce__]
-let repr_of_steel (#a : Type) (#req : req_t) (#ens : ens_t a) ($f : repr_steel_t a req ens)
+let repr_of_steel (#a : Type) (pre : pre_t) (post : post_t a) (req : req_t pre) (ens : ens_t pre a post)
+                  ($f : repr_steel_t a pre post req ens)
   : repr a
   = {
     repr_tree  = tree_of_steel f;
-    repr_steel = f
+    repr_steel = (fun pre' post' (|frame, p0, p1|) () ->
+        (**) steel_change_vequiv p0;
+        (**) steel_elim_vprop_of_list_append pre frame;
+        let x = f () in
+        (**) steel_intro_vprop_of_list_append (post x) frame;
+        (**) let sl1' = gget (vprop_of_list L.(post x @ frame)) in
+        (**) steel_change_vequiv (p1 x);
+        (**) let sl1'' = gget (vprop_of_list (post' x)) in
+        (**) assert (vpl_sels (post' x) sl1'' == extract_vars (p1 x) (vpl_sels L.(post x @ frame) sl1'));
+        (**) extract_vars_sym_l (p1 x) (vpl_sels L.(post x @ frame) sl1');
+        return x)
   }
 
 [@@ __tree_reduce__]
@@ -125,29 +608,43 @@ let return (#a : Type) (x :a)
   : repr a
   = {
     repr_tree  = Tret a x;
-    repr_steel = (fun () -> Steel.Effect.Atomic.return x)
+    repr_steel = (fun pre post p () ->
+        (**) steel_change_vequiv (Uv.downgrade_val p);
+        Steel.Effect.Atomic.return x)
   }
 
-let elim_tree_req_bind (#a #b : Type) (f : prog_tree a) (g : a -> prog_tree b) (sl0 : sl_t)
-  : Lemma (requires tree_req (Tbind a b f g) sl0)
-          (ensures  tree_req f sl0 /\
-                    (forall (x : a) (sl1 : sl_t) . tree_ens f sl0 x sl1 ==> tree_req (g x) sl1))
-  = assert_norm (tree_req (Tbind a b f g) sl0 == (
-      tree_req f sl0 /\
-      (forall (x : a) (sl1 : sl_t) . tree_ens f sl0 x sl1 ==> tree_req (g x) sl1)
+
+let elim_tree_req_bind (#a #b : Type) (f : prog_tree a) (g : a -> prog_tree b)
+      (#pre : pre_t) (#post : post_t b) (#itm : a -> vprop_list)
+      (cf  : tree_cond f pre itm) (cg : (x:a) -> tree_cond (g x) (itm x) post)
+      (sl0 : t_of (vprop_of_list pre))
+  : Lemma (requires tree_req (Tbind a b f g) (|itm, cf, cg|) (vpl_sels pre sl0))
+          (ensures  tree_req f cf (vpl_sels pre sl0) /\
+                    (forall (x : a) (sl1 : t_of (vprop_of_list (itm x))) .
+                      tree_ens f cf (vpl_sels pre sl0) x (vpl_sels (itm x) sl1) ==>
+                      tree_req (g x) (cg x) (vpl_sels (itm x) sl1)))
+  = assert_norm (tree_req (Tbind a b f g) (|itm, cf, cg|) (vpl_sels pre sl0) == (
+      tree_req f cf (vpl_sels pre sl0) /\
+      (forall (x : a) (sl1 : sl_t (itm x)) .
+         tree_ens f cf (vpl_sels pre sl0) x sl1 ==> tree_req (g x) (cg x) sl1)
     ))
 
 let intro_tree_ens_bind (#a #b : Type) (f : prog_tree a) (g : a -> prog_tree b)
-      (sl0 : sl_t) (x : a) (sl1 : sl_t) (y : b) (sl2 : sl_t)
-  : Lemma (requires tree_req f sl0 /\
-                    tree_ens f sl0 x sl1 /\
-                    tree_ens (g x) sl1 y sl2)
-          (ensures  tree_ens (Tbind a b f g) sl0 y sl2)
-  = assert_norm (tree_ens (Tbind a b f g) sl0 y sl2 == (
-      tree_req f sl0 /\
-        (exists (x : a) (sl1 : sl_t) .
-          tree_ens f sl0 x sl1 /\
-          tree_ens (g x) sl1 y sl2)
+      (#pre : pre_t) (#post : post_t b) (#itm : a -> vprop_list)
+      (cf  : tree_cond f pre itm) (cg : (x:a) -> tree_cond (g x) (itm x) post)
+      (sl0 : t_of (vprop_of_list pre)) (x : a) (sl1 : t_of (vprop_of_list (itm x)))
+      (y : b) (sl2 : t_of (vprop_of_list (post y)))
+  : Lemma (requires tree_req f cf (vpl_sels pre sl0) /\
+                    tree_ens f cf (vpl_sels pre sl0) x (vpl_sels (itm x) sl1) /\
+                    tree_ens (g x) (cg x) (vpl_sels (itm x) sl1) y (vpl_sels (post y) sl2))
+          (ensures  tree_ens (Tbind a b f g) #pre #post (|itm, cf, cg|)
+                             (vpl_sels pre sl0) y (vpl_sels (post y) sl2))
+  = assert_norm (tree_ens (Tbind a b f g) #pre #post (|itm, cf, cg|)
+                          (vpl_sels pre sl0) y (vpl_sels (post y) sl2) == (
+      tree_req f cf (vpl_sels pre sl0) /\
+        (exists (x : a) (sl1 : sl_t (itm x)) .
+          tree_ens f cf (vpl_sels pre sl0) x sl1 /\
+          tree_ens (g x) (cg x) sl1 y (vpl_sels (post y) sl2))
     ))
 
 [@@ __tree_reduce__]
@@ -156,37 +653,52 @@ let bind (#a #b : Type)
   : repr b
   = {
     repr_tree  = Tbind a b f.repr_tree (fun x -> (g x).repr_tree);
-    repr_steel = (fun () -> (**) let sl0 = gget vp in
-                         (**) elim_tree_req_bind f.repr_tree (fun x -> (g x).repr_tree) sl0;
-                         let x = f.repr_steel () in
-                         (**) let sl1 = gget vp in
-                         let y = (g x).repr_steel () in
-                         (**) let sl2 = gget vp in
-                         (**) intro_tree_ens_bind f.repr_tree (fun x -> (g x).repr_tree)
-                         (**)                     sl0 x sl1 y sl2;
-                         Steel.Effect.Atomic.return y)
+    repr_steel = (fun pre post (|itm, cf, cg|) () ->
+        (**) let sl0 = gget (vprop_of_list pre) in
+        (**) assert (tree_req (Tbind a b f.repr_tree (fun x -> (g x).repr_tree))
+        (**)                  (|itm, cf, cg|) (vpl_sels pre sl0));
+        (**) elim_tree_req_bind f.repr_tree (fun x -> (g x).repr_tree) cf cg sl0;
+        let x = f.repr_steel pre itm cf () in
+        (**) let sl1 = gget (vprop_of_list (itm x)) in
+        (**) assert (tree_ens f.repr_tree cf (vpl_sels pre sl0) x (vpl_sels (itm x) sl1));
+        (**) assert (tree_req (g x).repr_tree (cg x) (vpl_sels (itm x) sl1));
+        let y = (g x).repr_steel (itm x) post (cg x) () in
+        (**) let sl2 = gget (vprop_of_list (post y)) in
+        (**) intro_tree_ens_bind f.repr_tree (fun x -> (g x).repr_tree) cf cg
+        (**)                     sl0 x sl1 y sl2;
+        Steel.Effect.Atomic.return y)
   }
 
 (* --------------------------- *)
 
-module T = FStar.Tactics
-
-let read_req : req_t   = fun sl0 -> True
-let read_ens : ens_t nat = fun sl0 x sl1 -> sl1 == sl0 /\ x == Ghost.reveal sl0
-let read ()
-  : Steel nat vp (fun _ -> vp)
-      (requires fun h0     -> read_req (h0 vp))
-      (ensures fun h0 x h1 -> read_ens (h0 vp) x (h1 vp))
-  = read some_ref
-
-unfold let r_read : repr nat =
-  repr_of_steel #nat #read_req #read_ens read
+open Steel.FractionalPermission
+open Steel.Reference
 
 unfold
-let test : repr int =
-  x <-- r_read;
-  y <-- r_read;
-  return (x - y)
+let read_pre  (r : ref nat) : pre_t
+  = [vptr' r full_perm]
+unfold
+let read_post (r : ref nat) : post_t nat
+  = fun _ -> [vptr' r full_perm]
+let read_req  (r : ref nat) : req_t (read_pre r)
+  = fun sl0 -> True
+let read_ens  (r : ref nat) : ens_t (read_pre r) nat (read_post r)
+  = fun sl0 x sl1 -> var_at sl1 0 == var_at sl0 0 /\ x == var_at sl0 0
+
+let steel_read (r : ref nat)
+  : repr_steel_t nat (read_pre r) (read_post r) (read_req r) (read_ens r)
+  = fun () -> (**) change_equal_slprop (vprop_of_list (read_pre r)) (vptr r `star` emp);
+           let x = read r in
+           (**) change_equal_slprop (vptr r `star` emp) (vprop_of_list (read_post r x));
+           Steel.Effect.Atomic.return x
+
+unfold let r_read (r : ref nat) : repr nat =
+  repr_of_steel (read_pre r) (read_post r) (read_req r) (read_ens r) (steel_read r)
+
+unfold
+let test (r : ref nat) : repr nat =
+  x <-- r_read r;
+  return x
 
 irreducible
 let print_util (#a : Type) (x : a) : prop = True
@@ -198,8 +710,42 @@ let normal_tree_steps : list norm_step = [
     iota; zeta
   ]
 
-//let _ = assert (print_util test.repr_tree) by T.(norm normal_tree_steps; qed ())
+let normal_tree_cond_steps : list norm_step = [
+    delta_attr [`%__tree_reduce__];
+    delta_qualifier ["unfold"];
+    delta_only [`%Mkrepr?.repr_tree; `%tree_cond; `%tree_of_steel];
+    iota; zeta
+  ]
 
+let normal_spec_steps : list norm_step = [
+    delta; iota; zeta; primops
+  ]
+
+
+//let _ = fun r ->
+//  assert (print_util (test r).repr_tree) by T.(norm normal_tree_steps; qed ())
+
+unfold
+let test_cond (r : ref nat)
+  : norm normal_tree_cond_steps (tree_cond (test r).repr_tree [vptr' r full_perm] (fun _ -> [vptr' r full_perm]))
+  = (|(fun _ -> [vptr' r full_perm]),
+       (| [], Perm.id_n 1, (fun (_:nat) -> Perm.id_n 1) |), (fun _ -> Uv.raise_val (Perm.id_n 1))|)
+
+unfold
+let cast_unorm (s : list norm_step) (#t : Type) (x : norm s t) : t
+  = norm_spec s t; x
+
+unfold
+let cast_norm (s : list norm_step) (#t : Type) (x : t) : norm s t
+  = norm_spec s t; x
+
+//let _ = fun r ->
+//  assert (print_util (tree_req (test r).repr_tree
+//                     #[vptr' r full_perm] #(fun _ -> [vptr' r full_perm])
+//                     (cast_unorm normal_tree_cond_steps (test_cond r))))
+//    by T.(norm normal_spec_steps; qed ())
+
+(*
 (* --------------------------- *)
 
 /// generating a non-deterministic function representing the program tree
@@ -261,4 +807,5 @@ let normal_tree_ND_steps : list norm_step = [
 (*
 let _ = assert (print_util (prog_tree_to_ND (test.repr_tree)))
           by T.(norm (normal_tree_ND_steps); qed ())
+*)
 *)
